Better Skolemization predicate & upgrade notation for \\models

theories/Semantics.v
@@ -120,10 +120,10 @@ Arguments Model : clear implicits.
 Arguments Interpret {_ _ _} _ _ _.
 Arguments interpret {_ _ _} _ {_ _ _} _ _ _.
 
-Notation "\models F" := (is_valid F) (at level 40).
-Notation "[[ M # rho # sigma '\models F ]]" := (interpret M rho sigma F).
+Notation "|= F" := (is_valid F) (at level 40).
+Notation "[[ M # rho # sigma '|= F ]]" := (interpret M rho sigma F).
 Notation "F \equiv G" := (equiv F G) (at level 30).
-Notation "Gamma \models F" := (is_valid (Or (Neg (ls_to_form Gamma)) F)) (at level 40).
+Notation "Gamma |= F" := (is_valid (Or (Neg (ls_to_form Gamma)) F)) (at level 40).
 
 Section SemanticsFacts.
   Context {pred func var : Atom} `{set_nat : set nat}.
@@ -150,7 +150,7 @@ Section SemanticsFacts.
 
   Lemma is_satisfiable_is_not_countersat :
     forall (F : Form),
-      is_satisfiable F -> \models Neg F -> False.
+      is_satisfiable F -> |= Neg F -> False.
   Proof using Type.
     intros F hsat hfalse. destruct hsat as (M & hsat).
     specialize (hfalse M); specialize (hsat (empty_env M var)).
@@ -167,7 +167,7 @@ Section SemanticsFacts.
 
   Lemma in_form_list_models :
     forall (F : Form) (Gamma : list Form),
-      List.In F Gamma -> Gamma \models F.
+      List.In F Gamma -> Gamma |= F.
   Proof using Type.
     intros ?? Hin. induction Gamma as [|G Gs IHGs]; inversion Hin.
     - rewrite !H in IHGs |- *.
@@ -180,7 +180,7 @@ Section SemanticsFacts.
 
   Lemma explosion_principle :
     forall (F : Form) (Gamma : list Form),
-      Gamma \models Bot -> Gamma \models F.
+      Gamma |= Bot -> Gamma |= F.
   Proof using Type.
     intros F Gamma Hmodels M. cbn.
     specialize (Hmodels M). cbn in Hmodels. destruct Hmodels as [H | contra].
@@ -190,7 +190,7 @@ Section SemanticsFacts.
 
   Lemma models_iff :
     forall (F : Form) (Gamma : list Form),
-      (Gamma \models F) <-> ((Neg F :: Gamma) \models Bot).
+      (Gamma |= F) <-> ((Neg F :: Gamma) |= Bot).
   Proof using Type.
     intros F Gamma. split.
     - intros Hmodels M; cbn. specialize (Hmodels M). cbn in Hmodels.
@@ -205,7 +205,7 @@ Section SemanticsFacts.
 
   Lemma models_P_neg_P :
     forall (F : Form) (Gamma : list Form),
-      Gamma \models F -> Gamma \models Neg F -> Gamma \models Bot.
+      Gamma |= F -> Gamma |= Neg F -> Gamma |= Bot.
   Proof using Type.
     intros F Gamma HF HNF M.
     specialize (HF M); specialize (HNF M); cbn in HF, HNF |- *.
@@ -215,7 +215,7 @@ Section SemanticsFacts.
   Lemma in_form_list_interp :
     forall {F : Form} {Gamma : list Form} {M : Model pred func}
       {rho : list M} {sigma : env M var},
-      List.In F Gamma -> [[ M # rho # sigma '\models ls_to_form Gamma ]] -> [[ M # rho # sigma '\models F ]].
+      List.In F Gamma -> [[ M # rho # sigma '|= ls_to_form Gamma ]] -> [[ M # rho # sigma '|= F ]].
   Proof using Type.
     intros ????? hin hinterp; induction Gamma as [|G Gs IHGs]; inversion hin; subst.
     - cbn in hinterp |- *. apply NNPP => save. apply hinterp; now left.
@@ -225,8 +225,8 @@ Section SemanticsFacts.
   Lemma extend_with_equiv_form :
     forall (F G : Form) (Gamma : list Form) (M : Model pred func)
       (rho : list M) (sigma : env M var),
-      [[ M # rho # sigma '\models ls_to_form Gamma ]] -> F \equiv G -> List.In G Gamma ->
-      [[ M # rho # sigma '\models ls_to_form (F :: Gamma) ]].
+      [[ M # rho # sigma '|= ls_to_form Gamma ]] -> F \equiv G -> List.In G Gamma ->
+      [[ M # rho # sigma '|= ls_to_form (F :: Gamma) ]].
   Proof using Type.
     intros ?????? hinterp hequiv hin. cbn. intros [hnF | hnG]; auto.
     have hG := in_form_list_interp hin hinterp.
@@ -237,37 +237,19 @@ Section SemanticsFacts.
   Lemma extend_with_imply_form :
     forall (F G : Form) (Gamma : list Form) (M : Model pred func)
       (sigma : env M var),
-      [[ M # [] # sigma '\models ls_to_form Gamma ]] -> imply G F -> List.In G Gamma ->
-      [[ M # [] # sigma '\models ls_to_form (F :: Gamma) ]].
+      [[ M # [] # sigma '|= ls_to_form Gamma ]] -> imply G F -> List.In G Gamma ->
+      [[ M # [] # sigma '|= ls_to_form (F :: Gamma) ]].
   Proof using Type.
     intros ????? hinterp himply hin. cbn. intros [hnF | hnG]; auto.
     have hG := in_form_list_interp hin hinterp.
     now apply hnF, himply.
   Qed.
 
-  Lemma extend_with_imply_form' :
-    forall (F G : Form) (Gamma : list Form) (M : Model pred func)
-      (sigma : env M var),
-      [[ M # [] # sigma '\models ls_to_form Gamma ]] ->
-      ((~ [[ M # [] # sigma '\models F ]]) ->
-       exists M' sigma',
-         (~ [[ M' # [] # sigma' '\models G ]]) /\
-           [[ M' # [] # sigma' '\models ls_to_form Gamma ]]) ->
-      List.In G Gamma -> [[ M # [] # sigma '\models ls_to_form (F :: Gamma) ]].
-  Proof using Type.
-    intros ????? hinterp himply hin. cbn. intros [hnF | hnG]; auto.
-    have hG := in_form_list_interp hin hinterp.
-    specialize (himply hnF). destruct himply as (M' & sigma' & h); auto.
-    destruct h as (hnG & hGamma) .
-    have h := in_form_list_interp hin hGamma.
-    now apply hnG.
-  Qed.
-
   Lemma interp_list_commute :
     forall (F G : Form) (Gamma : list Form) (M : Model pred func)
       (rho : list M) (sigma : env M var),
-      [[ M # rho # sigma '\models ls_to_form (Neg (Or (Neg F) (Neg G)) :: Gamma) ]] ->
-      [[ M # rho # sigma '\models ls_to_form (F :: G :: Gamma) ]].
+      [[ M # rho # sigma '|= ls_to_form (Neg (Or (Neg F) (Neg G)) :: Gamma) ]] ->
+      [[ M # rho # sigma '|= ls_to_form (F :: G :: Gamma) ]].
   Proof using Type.
     intros ?????? hinterp. cbn in *. intros [hnF | hinterp'].
     - apply hinterp. left. intros h; apply h. now left.
@@ -333,7 +315,7 @@ Section SemanticsFacts.
     forall (M : Model pred func) (rho : list M) (sigma : env M var) (t u : Term),
       isLocallyClosed u ->
       interpret_term M rho sigma (t {#|rho| \to u}) =
-        interpret_term M (rho ++ [ [[ M # rho # sigma '\models u ]] ])%list sigma t.
+        interpret_term M (rho ++ [ [[ M # rho # sigma '|= u ]] ])%list sigma t.
   Proof using Type.
     intros ??????. induction t using term_ind.
     - cbn. rewrite -match_eq_dec_eq_bool; destruct (#|rho| == n).
@@ -349,7 +331,7 @@ Section SemanticsFacts.
             cbn in H0. lia. }
           rewrite nth_error_app1; auto.
           now rewrite e.
-        * have hgt : #|rho ++ [ [[ M # rho # sigma '\models u ]] ]|  <= n.
+        * have hgt : #|rho ++ [ [[ M # rho # sigma '|= u ]] ]|  <= n.
           { rewrite nth_error_None in e.
             have hlt : #|rho| < n by lia.
             rewrite last_length. lia. }
@@ -358,7 +340,7 @@ Section SemanticsFacts.
     - now cbn.
     - cbn. rewrite map_map.
       have hmap : (map (fun x : Term_ func var => interpret_term M rho sigma x {#| rho | \to u}) l) =
-                    (map (interpret_term M (rho ++ [ [[M # rho # sigma '\models u]] ])%list sigma) l).
+                    (map (interpret_term M (rho ++ [ [[M # rho # sigma '|= u]] ])%list sigma) l).
       { induction l as [|v vs IHvs]; auto; cbn.
         rewrite IHvs.
         - now apply Forall_tail in X.
@@ -372,12 +354,12 @@ Section SemanticsFacts.
     forall (M : Model pred func) (rho : list M) (sigma : env M var) (F : Form) (t : Term),
       isLocallyClosed t ->
       interpret_form_ M rho sigma (F {#|rho| \to t}) =
-        interpret_form_ M (rho ++ [ [[ M # rho # sigma '\models t ]] ])%list sigma F.
+        interpret_form_ M (rho ++ [ [[ M # rho # sigma '|= t ]] ])%list sigma F.
   Proof using Type.
     intros ??????. revert rho. induction F; auto; cbn; intros rho.
     - rewrite map_map.
       have hmap : (map (fun u => interpret_term M rho sigma u {#|rho| \to t}) l) =
-                    (map (interpret_term M (rho ++ [ [[ M # rho # sigma '\models t ]] ])%list sigma) l).
+                    (map (interpret_term M (rho ++ [ [[ M # rho # sigma '|= t ]] ])%list sigma) l).
       { induction l as [|v vs IHvs]; auto; cbn.
         rewrite IHvs term_env_inst_commutes; auto. }
       rewrite hmap //.
@@ -404,12 +386,12 @@ Section SemanticsFacts.
 
   Definition subst_to_env (M : Model pred func)
     (sigma : Substitution var Term) : env M var :=
-    fun x => Some ([[ M # [] # empty_env M var '\models sigma x ]]).
+    fun x => Some ([[ M # [] # empty_env M var '|= sigma x ]]).
 
   Lemma subst_commutes_with_env_terms :
     forall (M : Model pred func) (t : Term) (rho : list M) (sigma : Substitution var Term),
-      [[ M # rho # empty_env M var '\models t@[sigma] ]] =
-        [[ M # rho # subst_to_env M sigma '\models t ]].
+      [[ M # rho # empty_env M var '|= t@[sigma] ]] =
+        [[ M # rho # subst_to_env M sigma '|= t ]].
   Proof using Type.
     intros. induction t using term_ind; cbn; try reflexivity.
     - apply isLocallyClosed_interp_env. apply isSubst.
@@ -421,8 +403,8 @@ Section SemanticsFacts.
 
   Lemma subst_commutes_with_env_forms :
     forall (M : Model pred func) (F : Form) (rho : list M) (sigma : Substitution var Term),
-      [[ M # rho # empty_env M var '\models F@[sigma] ]] <->
-        [[ M # rho # subst_to_env M sigma '\models F ]].
+      [[ M # rho # empty_env M var '|= F@[sigma] ]] <->
+        [[ M # rho # subst_to_env M sigma '|= F ]].
   Proof using Type.
     intros M F. induction F; cbn.
     - reflexivity.
@@ -431,8 +413,8 @@ Section SemanticsFacts.
                  map (interpret_term M rho (subst_to_env M sigma)) l.
       { induction l as [|t ts IHts]; cbn; auto.
         rewrite IHts. f_equal.
-        change ([[ M # rho # empty_env M var '\models t@[sigma] ]] =
-                  [[ M # rho # subst_to_env M sigma '\models t ]]).
+        change ([[ M # rho # empty_env M var '|= t@[sigma] ]] =
+                  [[ M # rho # subst_to_env M sigma '|= t ]]).
         apply subst_commutes_with_env_terms. }
       now rewrite e.
     - intros ??. rewrite IHF //.
