.dir-locals.el
@@ -4,7 +4,7 @@
 ((coq-mode . ((company-coq-dir-local-symbols . (("\\to" . ?→)
 												("\\in" . ?∈)
 												("\\subseteq" . ?⊆)
-												("\\models" . ?⊧)
+												("|=" . ?⊧)
 												("[[" . ?〚)
 												("]]" . ?〛)
 												("Gamma" . ?Γ)
